commit

AP/Sokoban/Card.lean
@@ -2,17 +2,102 @@ import AP.Sokoban.Basic
 
 namespace Sokoban
 
-private structure FinState (w h : ℕ) where
-  mp : Map (Fin w × Fin h) Tile
+theorem point_eq_of_fin {s : State} [hs : s.Valid] {p : PointZ}
+(h : p ∈ s.grid) : p = ⟨(p.x.toFin : Fin s.width), (p.y.toFin : Fin s.height)⟩ := by
+  rcases p with ⟨x, y⟩
+  simp
+  simp [hs.h_bounds] at h
+  rcases h with ⟨h₁, h₂, h₃, h₄⟩
+  rw [eq_comm]; nth_rw 2 [eq_comm]
+  simp [Int.toFin, Nat.toFin]
+  rw [max_eq_left h₁, max_eq_left h₂]
+  exact ⟨Int.emod_eq_of_lt h₁ h₃, Int.emod_eq_of_lt h₂ h₄⟩
+
+theorem x_toFin_width_eq_iff' {s : State} [hs : s.Valid] {p₁ p₂ : PointZ}
+(h₁ : p₁ ∈ s.grid) (h₂ : p₂ ∈ s.grid) :
+(p₁.x.toFin : Fin s.width) = p₂.x.toFin ↔ p₁.x = p₂.x := by
+  nth_rw 2 [point_eq_of_fin h₁, point_eq_of_fin h₂]; simp [Fin.ext_iff]
+
+theorem y_toFin_width_eq_iff' {s : State} [hs : s.Valid] {p₁ p₂ : PointZ}
+(h₁ : p₁ ∈ s.grid) (h₂ : p₂ ∈ s.grid) :
+(p₁.y.toFin : Fin s.height) = p₂.y.toFin ↔ p₁.y = p₂.y := by
+  nth_rw 2 [point_eq_of_fin h₁, point_eq_of_fin h₂]; simp [Fin.ext_iff]
+
+theorem x_toFin_width_eq_iff {n} [hn : NeZero n] {s₁ s₂ : State}
+[hs₁ : s₁.Valid] [hs₂ : s₂.Valid] {p₁ p₂}
+(hw₁ : s₁.width = n) (hw₂ : s₂.width = n) (h₁ : p₁ ∈ s₁.grid) (h₂ : p₂ ∈ s₂.grid) :
+(p₁.x.toFin : Fin n) = p₂.x.toFin ↔ p₁.x = p₂.x := by
+  nth_rw 2 [point_eq_of_fin h₁, point_eq_of_fin h₂]; simp [Fin.ext_iff]
+  congr!; exact hw₁.symm; exact hw₂.symm
+
+theorem y_toFin_width_eq_iff {n} [hn : NeZero n] {s₁ s₂ : State}
+[hs₁ : s₁.Valid] [hs₂ : s₂.Valid] {p₁ p₂}
+(hw₁ : s₁.height = n) (hw₂ : s₂.height = n) (h₁ : p₁ ∈ s₁.grid) (h₂ : p₂ ∈ s₂.grid) :
+(p₁.y.toFin : Fin n) = p₂.y.toFin ↔ p₁.y = p₂.y := by
+  nth_rw 2 [point_eq_of_fin h₁, point_eq_of_fin h₂]; simp [Fin.ext_iff]
+  congr!; exact hw₁.symm; exact hw₂.symm
+
+private structure FinState (w h : ℕ) [NeZero w] [NeZero h] where
+  grid : Map (Fin w × Fin h) Tile
   player : Fin w × Fin h
 deriving Fintype
 
--- private def State.supReach (s : State) : Finset State := List.toFinset do
---   let grid ← do
---   { s with
---     grid := grid
---   }
+private def fn (s₀ : State) [hs : s₀.Valid] (s : State) :
+FinState s₀.width s₀.height :=
+  { grid := Map.range # λ p => s.grid.get! ⟨p.1, p.2⟩
+    player := (s.player.x.toFin, s.player.y.toFin)
+  }
 
--- theorem finite_reachable {s : State} [hs : s.Valid] :
--- {s' | sys.Reachable s s'}.Finite := by
---   apply Set.finite_of_subset_finset (s := s.supReach)
+theorem finite_reachable {s : State} [hs : s.Valid] :
+{s' | sys.Reachable s s'}.Finite := by
+  rename' s => s₀
+  unfold Set.Finite
+  simp
+  apply Finite.of_injective # λ ⟨s, _⟩ => fn s₀ s
+  rintro ⟨s₁, hs₁⟩ ⟨s₂, hs₂⟩ h
+  simp [fn] at h
+  rcases h with ⟨h₁, h₂, h₃⟩
+  simp
+  have h₄ : s₁.Valid := valid_of_reachable hs₁
+  have h₅ : s₂.Valid := valid_of_reachable hs₂
+  ext:1
+  · rw [width_eq_of_reachable hs₁, width_eq_of_reachable hs₂]
+  · rw [height_eq_of_reachable hs₁, height_eq_of_reachable hs₂]
+  · clear h₂ h₃
+    ext p d
+    specialize h₁ p.x.toFin p.y.toFin
+    simp only [Map.get!_eq_get?_get!] at h₁
+    by_cases hp : p ∉ s₀.grid
+    · constructor <;> intro h₂ <;> replace h₂ := Map.mem_of_get?_eq_some h₂
+      · rw [mem_grid_iff_of_reachable hs₁] at h₂; contradiction
+      · rw [mem_grid_iff_of_reachable hs₂] at h₂; contradiction
+    simp at hp
+    have hp₁ := mem_grid_iff_of_reachable hs₁ |>.mpr hp
+    have hp₂ := mem_grid_iff_of_reachable hs₂ |>.mpr hp
+    have H₁ : (↑(p.x.toFin : Fin s₀.width) : ℕ) = p.x
+    · nth_rw 2 [point_eq_of_fin hp₁]; simp
+      apply Int.toFin_congr; symm; exact width_eq_of_reachable hs₁; rfl
+    have H₂ : (↑(p.y.toFin : Fin s₀.height) : ℕ) = p.y
+    · nth_rw 2 [point_eq_of_fin hp₁]; simp
+      apply Int.toFin_congr; symm; exact height_eq_of_reachable hs₁; rfl
+    rw [H₁, H₂] at h₁; clear H₁ H₂ hp hp₁ hp₂
+    rcases p with ⟨x, y⟩
+    simp at h₁ ⊢
+    constructor <;> intro h₂
+    · simp [h₂] at h₁
+      subst h₁
+      simp
+      rw [mem_grid_iff_of_reachable hs₂]
+      rw [←mem_grid_iff_of_reachable hs₁]
+      apply Map.mem_of_get?_eq_some h₂
+    · simp [h₂] at h₁
+      subst h₁
+      simp
+      rw [mem_grid_iff_of_reachable hs₁]
+      rw [←mem_grid_iff_of_reachable hs₂]
+      apply Map.mem_of_get?_eq_some h₂
+  · rw [x_toFin_width_eq_iff (width_eq_of_reachable hs₁)
+      (width_eq_of_reachable hs₂) player_mem player_mem] at h₂
+    rw [y_toFin_width_eq_iff (height_eq_of_reachable hs₁)
+      (height_eq_of_reachable hs₂) player_mem player_mem] at h₃
+    ext <;> assumption
