AP/Util/Fin.lean
@@ -9,3 +9,16 @@ def next {n} (k : Fin n) : Fin n := by
 
 theorem toNat_next_eq {n} {k : Fin n} :
 k.next.toNat = if k.toNat + 1 = n then 0 else k.toNat + 1 := by rfl
+
+end Fin
+
+def Nat.toFin (k : ℕ) {n} [NeZero n] : Fin n := Fin.ofNat _ k
+def Int.toFin (k : ℤ) {n} [NeZero n] : Fin n := k.toNat.toFin
+
+theorem Nat.toFin_congr {n m} [hn : NeZero n] [hm : NeZero m] {k₁ k₂ : ℕ}
+(h₁ : n = m) (h₂ : k₁ = k₂) : (↑(k₁.toFin : Fin n) : ℕ) = (↑(k₂.toFin : Fin m) : ℕ) := by
+  subst h₁ h₂; rfl
+
+theorem Int.toFin_congr {n m} [hn : NeZero n] [hm : NeZero m] {k₁ k₂ : ℤ}
+(h₁ : n = m) (h₂ : k₁ = k₂) : (↑(k₁.toFin : Fin n) : ℕ) = (↑(k₂.toFin : Fin m) : ℕ) := by
+  subst h₁ h₂; rfl
