AP/System/Invariant.lean
@@ -7,7 +7,7 @@ variable {S T : Type u} {sys : System S T}
 
 theorem invariant {p : S → Prop} {a b}
 (h₁ : p a) (h₂ : sys.Reachable a b)
-(h₃ : ∀ {x t y}, p x → sys.trTo x t y → p y) : p b := by
+(h₃ : ∀ {x y t}, p x → sys.trTo x t y → p y) : p b := by
   induction h₂; exact h₁
   clear a b
   nm a b c t h₂ h₄ ih
@@ -20,3 +20,10 @@ theorem invariant_init {p : S → Prop} {a}
   rw [valid_iff] at h₁
   obtain ⟨s₀, h₁, h₄⟩ := h₁
   exact invariant (h₂ h₁) h₄ h₃
+
+theorem invariant_val {α : Type*} {a b} {f : S → α} (h₁ : sys.Reachable a b)
+(h₂ : ∀ {x y t}, sys.trTo x t y → f y = f x) : f b = f a := by
+  apply invariant (p := (f · = f a)) rfl h₁
+  intro x y t h₃ h₄
+  rw [←h₃]
+  exact h₂ h₄
